aaaaaa

LeanSAT/Model/PropAssn.lean
@@ -182,7 +182,7 @@ theorem pmap_pmap {P : ν₂ → Prop} [DecidablePred P] {Q : ν₁ → Prop} [D
 
 def preimage [Fintype ν₁] [DecidableEq ν₂] (f : ν₁ ↪ ν₂) (τ : PropAssignment ν₁)
     : PropAssignment ν₂ :=
-  pmap (fun ⟨v2,h⟩ => (Finset.mapEquiv Finset.univ f).symm ⟨v2,h⟩) τ
+  pmap (fun ⟨v2,h⟩ => Fintype.invFun f ⟨v2,h⟩) τ
 
 theorem get_preimage [Fintype ν₁] [DecidableEq ν₂] (f : ν₁ ↪ ν₂) {τ v v'}
     : v = f.1 v' → (preimage f τ) v = τ v' := by
@@ -192,3 +192,10 @@ theorem get_preimage [Fintype ν₁] [DecidableEq ν₂] (f : ν₁ ↪ ν₂) {
 theorem map_preimage [Fintype ν₁] [DecidableEq ν₂] (f : ν₁ → ν₂) (f') (τ)
     : f = f'.1 → map f (preimage f' τ) = τ := by
   rintro rfl; ext v1; simp [preimage]
+
+@[simp]
+theorem preimage_map [Fintype ν₁] [Fintype ν₃] [DecidableEq ν₂] [DecidableEq ν₃] (f : ν₁ ↪ ν₂) (f' : ν₁ ↪ ν₃) (τ)
+    : preimage f (map f' τ) = map (sorry) τ := by
+  simp [preimage]; rw [get_pmap]
+  simp [*]
+  assumption
